lib/BPFStar.RingBuf.fst
@@ -8,6 +8,9 @@ open Pulse.Lib.Pervasives
 open FStar.Ghost
 
 let bpf_ringbuf = unit
+
+let define_ringbuf _ = admit ()
+
 let ringbuf_perm _ = emp
 let ringbuf_reservation #_ _ = emp
 
